specs/ecdsap256/Spec.ECC.Curves.fst
@@ -220,3 +220,11 @@ let basePoint #curve : point_nat_prime #curve  =
    |P384 -> assert_norm(0xaa87ca22be8b05378eb1c71ef320ad746e1d3b628ba79b9859f741e082542a385502f25dbf55296c3a545e3872760ab7 < getPrime P384);
   (0xaa87ca22be8b05378eb1c71ef320ad746e1d3b628ba79b9859f741e082542a385502f25dbf55296c3a545e3872760ab7,0x3617de4a96262c6f5d9e98bf9292dc29f8f41dbd289a147ce9da3113b5f0b8c00a60b1ce1d7e819d7a431d7c90ea0e5f, 1) 
 
+
+val isPrimeGroup: c: curve -> Tot bool
+
+let isPrimeGroup c = 
+  match c with 
+  |P256 -> true
+  |P384 -> true
+  |_ -> false
